examples/crypto/cryptobox/Box.DH.fst
@@ -4,6 +4,7 @@
 *)
 module Box.DH
 
+open FStar.Set
 open FStar.HyperHeap
 open FStar.HyperStack
 open FStar.Monotonic.RRef
@@ -20,6 +21,8 @@ open Box.Flags
 
 module MR = FStar.Monotonic.RRef
 module MM = MonotoneMap
+module HS = FStar.HyperStack
+module HH = FStar.HyperHeap
 
 
 assume val dh_element_size : nat
@@ -41,7 +44,7 @@ assume val hash: dh_element -> Tot aes_key
 private type range = fun (k_id:ae_id) -> k:PlainDH.key{PlainDH.ae_key_get_index k = k_id}
 private let inv (f:MM.map' (ae_id) range) = True
 
-assume val ae_key_log_region: (r:MR.rid{ extends r root /\ is_eternal_region r /\ is_below r root})
+assume val ae_key_log_region: (r:HH.rid{ extends r root /\ is_eternal_region r /\ is_below r root /\ disjoint r id_table_region /\ disjoint r ae_key_region})
 //private let ae_key_log_region = new_region root
 assume val ae_key_log: MM.t ae_key_log_region ae_id range inv
 //private let ae_key_log = MM.alloc #ae_key_log_region #ae_id #range #inv
@@ -85,6 +88,7 @@ let coerce_keypair #i dh_ex =
   pk,sk
 
 
+// Make this function GTot
 val prf_odhT: dh_skey -> dh_pkey -> Tot aes_key
 let prf_odhT dh_sk dh_pk =
   let pk_id = dh_pk.pk_id in
@@ -94,6 +98,9 @@ let prf_odhT dh_sk dh_pk =
   let k = hash raw_k in
   k
   
+
+
+let s:Set.set (r:HH.rid) = Set.union (Set.singleton ae_key_log_region) (Set.singleton ae_key_region)
 
 (**
    If we prf_odh is true, the output of this function is random, if both 
@@ -111,8 +118,8 @@ val prf_odh: sk:dh_skey -> pk:dh_pkey -> ST (PlainDH.key)
     /\ (ae_honest i \/ ae_dishonest i)
     /\ (
         ( (ae_honest i /\ prf_odh)
-	    ==> (
-	       MR.witnessed (MM.contains ae_key_log i k) 
+	    ==> (True//modifies s h0 h1
+	       /\ MR.witnessed (MM.contains ae_key_log i k) 
 	      )
         )
         \/ 
@@ -123,7 +130,10 @@ val prf_odh: sk:dh_skey -> pk:dh_pkey -> ST (PlainDH.key)
         )
       )
   ))
+
+// Prove memory-safety for prf_odh
 let prf_odh dh_sk dh_pk =
+  let h0 = ST.get() in
   let pk_id = dh_pk.pk_id in
   let sk_id = dh_sk.sk_id in
   let i = generate_ae_id pk_id sk_id in
@@ -135,7 +145,10 @@ let prf_odh dh_sk dh_pk =
     | Some  k' -> k'
     | None -> 
       let k' = PlainDH.keygen i in
+      // For some reason, extend violates modifies ... maybe separate regions better?
       MM.extend ae_key_log i k';
+      let h1 = ST.get() in
+      assert(modifies s h0 h1);
       k')
   else(
     assert(ae_dishonest i \/ ~prf_odh);
